start working on Pack25519

Low/Pack25519.v
@@ -1,6 +1,8 @@
 From Tweetnacl Require Import Libs.Export.
 From Tweetnacl Require Import ListsOp.Export.
-Require Import stdpp.prelude.
+From Tweetnacl Require Import Mid.SubList.
+From stdpp Require Import prelude.
+Require Import Recdef.
 
 (*
 sv pack25519(u8 *o,const gf n)
@@ -13,10 +15,12 @@ sv pack25519(u8 *o,const gf n)
   car25519(t);
   FOR(j,2) {
     m[0]=t[0]-0xffed;
+
     for(i=1;i<15;i++) {
       m[i]=t[i]-0xffff-((m[i-1]>>16)&1);
       m[i-1]&=0xffff;
     }
+
     m[15]=t[15]-0x7fff-((m[14]>>16)&1);
     b=(m[15]>>16)&1;
     m[14]&=0xffff;
@@ -30,7 +34,58 @@ sv pack25519(u8 *o,const gf n)
 *)
 
 Open Scope Z.
+(*
+0xffff = 65535
+0xffed = 65517
+0x7fff = 32767
+*)
 
-Definition subst_65535 n m := n - 65535 - (Z.land (Z.shiftr m 16) 1).
+Definition subst_0xffed t := t - 65517.
+Definition subst_0xffff t m := t - 65535 - (Z.land (Z.shiftr m 16) 1).
+Definition subst_0x7fff t m := t - 32767 - (Z.land (Z.shiftr m 16) 1).
+Definition mod0xffff m := Z.land m 65535.
+Definition getBit256 l := Z.land (Z.shiftr (nth 15%nat l 0) 16) 1.
+
+Definition step_sub (a:Z) (m t:list Z) : list Z :=
+    let m' := nth (Z.to_nat (a - 1)) m 0 in
+    let t' := nth (Z.to_nat a) t 0 in
+      upd_nth (Z.to_nat (a-1)) (upd_nth (Z.to_nat a) m (subst_0xffff t' m')) (mod0xffff m').
+
+Function sub_fn_rev (a:Z) (m t: list Z) {measure Z.to_nat a} : (list Z) :=
+  if (a <=? 0)
+    then m
+    else
+      let prev := sub_fn_rev (a - 1) m t in 
+        step_sub a prev t.
+Proof. intros. apply Z2Nat.inj_lt ; move: teq ; rewrite Z.leb_gt => teq; omega. Defined.
+
+Lemma sub_fn_rev_0 : forall m t,
+  sub_fn_rev 0 m t = m.
+Proof. go. Qed.
+
+Lemma sub_fn_rev_n : forall a m t,
+  0 < a ->
+  sub_fn_rev a m t = step_sub a (sub_fn_rev (a - 1) m t) t.
+Proof. intros. rewrite sub_fn_rev_equation.
+flatten ; apply Zle_bool_imp_le in Eq; omega.
+Qed.
+
+Definition m_from_t (m t:list Z) : list Z := 
+  let m0 := upd_nth 0 m (subst_0xffed (nth 0 t 0)) in
+  let m14 := sub_fn_rev 14 m0 t in
+  let m15 := upd_nth 15 m14 (subst_0x7fff (nth 15 t 0) (nth 14 m14 0)) in
+  upd_nth 14 m15 (mod0xffff (nth 14 m15 0)).
+
+(*
+Definition list25519 := [65517;65535;65535;65535;65535;65535;65535;65535;65535;65535;65535;65535;65535;65535;65535;32767].
+Lemma list_of_P: forall l,
+  l = list25519 ->
+  (ZofList 16 l) = Z.pow 2 255 - 19.
+Proof. intros; subst; compute ; reflexivity. Qed.
+*)
+
+
+
+
 
 Close Scope Z.
